\documentclass[10pt,a4paper]{article}
\usepackage[utf8]{inputenc}
\usepackage[english]{babel}
\usepackage{amsmath}
\usepackage{amsfonts}
\usepackage{amssymb}
\usepackage{graphicx}
\usepackage[margin=0.5in]{geometry}
\usepackage{amsthm}
\usepackage{enumitem}
\newtheorem{question}{Question}
\newtheorem*{question*}{Question}
\newtheorem{answer}{Answer}
\newtheorem*{answer*}{Answer}
\newtheorem{theorem}{Theorem}
\newtheorem{lemma}{Lemma}

\title{Complex Analysis Homework 2}
\author{Colin Williams}

\begin{document}
\maketitle
\section*{Question 1}
\begin{question*}{$ $}
\\Show the following equations hold by writing the factors on the left in exponential form first:
\begin{enumerate}[label = \alph*.)]
\item $(\sqrt{3} + i)^6 = -64$
\item $(1 + \sqrt{3}i)^{-10} = 2^{-11}(-1 + \sqrt{3}i)$.
\end{enumerate}
\end{question*}

First, note that for $z \in \mathbb{C}$ expressed as $z = x + iy$ in rectangular form is equivalent to $z = r(cos(\theta) + i\sin(\theta))$ for $r = |z|$, $x = r\cos(\theta)$, and $y = r\sin(\theta)$ in polar form.\\
Also, note that $e^{i\theta} = \cos(\theta) + i\sin(\theta)$, so $z = re^{i\theta}$

\begin{proof}{\textbf{a.)}}
\\If $z = \sqrt{3} + i$, then, $r = |z| = \sqrt{(\sqrt{3})^2 + (1)^2} = 2$ and $\cos(\theta) = \sqrt{3}/2$ and $\sin(\theta) = 1/2 \implies \theta = \pi/6$\\
Thus,
\begin{align*}
z = re^{i\theta} &= 2e^{i(\pi/6)}\\
z^{6} &= (2e^{i(\pi/6)})^6\\
&= 2^6e^{i\pi}\\
&= 64(\cos(\pi) + i\sin(\pi))\\
&= 64(-1 + i(0))\\
z^6 = (\sqrt{3} + i)^6 &= -64
\end{align*}
which is our desired equality.
\end{proof}

\begin{proof}{\textbf{b.)}}
\\If $z = 1 + \sqrt{3}i$, then, $r = |z| = \sqrt{(1)^2 + (\sqrt{3})^2} = 2$ and $\cos(\theta) = 1/2$ and $\sin(\theta) = \sqrt{3}/2 \implies \theta = \pi/3$\\
Thus,
\begin{align*}
z = re^{i\theta} &= 2e^{i(\pi/3)}\\
z^{-10} &= (2e^{i(\pi/3)})^{-10}\\
&= 2^{-10}e^{i(-10\pi/3)}\\
&= 2^{-10}e^{i(-9\pi/3)}e^{i(-\pi/3)}\\
&= 2^{-10}e^{i(-3\pi)}e^{i(-\pi/3)}\\
&= 2^{-10}e^{i\pi}e^{i(-\pi/3)}\\
&= 2^{-10}(\cos(\pi) + i\sin(\pi))(\cos(-\frac{\pi}{3}) + i\sin(-\frac{\pi}{3}))\\
&= 2^{-10}(-1 + i(0))(\frac{1}{2} - i\frac{\sqrt{3}}{2})\\
&= 2^{-10}(-1)(\frac{1}{2})(1 - \sqrt{3}i)\\
z^{-10} = (1 + \sqrt{3}i)^{-10} &= 2^{-11}(-1 + \sqrt{3}i)
\end{align*}
which is our desired equality.
\end{proof}

\end{document}