\documentclass[10pt,a4paper]{article}
\usepackage[utf8]{inputenc}
\usepackage[english]{babel}
\usepackage{csquotes}
\usepackage{amsmath}
\usepackage{amsfonts}
\usepackage{amssymb}
\usepackage{graphicx}
\usepackage[margin=0.5in]{geometry}
\usepackage{amsthm}
\usepackage{enumitem}
\usepackage{tikz}
\usetikzlibrary{calc}
\newtheorem{question}{Question}
\newtheorem*{question*}{Question}
\newtheorem{theorem}{Theorem}
\newtheorem*{theorem*}{Theorem}
\newtheorem{lemma}{Lemma}

\theoremstyle{definition}
\newtheorem{answer}{Answer}
\newtheorem*{answer*}{Answer}


\title{Complex Analysis Homework 6}
\author{Colin Williams}

\begin{document}
\maketitle

\section*{Question 4}
Write down an expression of the form $\displaystyle \sum_{n = 0}^{\infty} a_nz^n$ for 
\begin{enumerate}[label = (\alph*)]
\item $\displaystyle \frac{1}{1 + z^4}$
\item $\displaystyle \frac{1}{2z + 5}$
\end{enumerate}
In each case, specify where the expansion is valid.
\\
\\To find these expansions, I will use the geometric series given by 
$\displaystyle \sum_{n = 0}^{\infty}w^n = \frac{1}{1 - w}$
for all $|w| < 1$.

\begin{answer*}{\textbf{(a)}}
\begin{align*}
\frac{1}{1 + z^4} &= \frac{1}{1 - (-z^4)}\\
&= \sum_{n = 0}^{\infty} (-z^4)^n\\
&= \boxed{\sum_{n = 0}^{\infty} (-1)^nz^{4n}}
\end{align*}
Since our $w$ in this case was equal to $-z^4$, this is valid whenever $|-z^4| < 1 \implies \boxed{|z| < 1}$
\\
\\Note, this is not quite in the form we desire since the exponent of $z$ is $4n$ instead of just $n$. However, if we re-define $a_n$ as the following:
\[
\begin{cases}
	a_n = 0 &\text{ if } n = 4k + m,\; m \in \{1,2,3\}\\
	a_n = (-1)^{k} &\text{ if } n = 4k
\end{cases}k \in \mathbb{Z}
\]
Then we get $\displaystyle \frac{1}{1 + z^4} = \sum_{n = 0}^{\infty} a_n z^n$ just as desired. However, I think the first answer is easier to work with.
\end{answer*}

\begin{answer*}{\textbf{(b)}}
\begin{align*}
\frac{1}{2z + 5} &= \frac{1}{5}\cdot \frac{1}{\displaystyle 1 + \frac{2z}{5}}\\
&= \frac{1}{5} \cdot \frac{1}{\displaystyle 1 - \left(-\frac{2z}{5}\right)}\\
&= \frac{1}{5}\sum_{n = 0}^{\infty} \left(-\frac{2z}{5}\right)^n\\
&= \boxed{\sum_{n = 0}^{\infty} \frac{(-2)^n}{5^{n+1}}z^n}
\end{align*}
Since our $w$ in this case was equal to $-\frac{2z}{5}$, this is valid whenever $\left|-\frac{2z}{5}\right| < 1 \implies \boxed{|z| < \frac{5}{2}}$
\\
\\Note this is the form we desired with $\displaystyle a_n = \frac{(-2)^n}{5^{n+1}}$.
\end{answer*}
\end{document}