\documentclass[10pt,a4paper]{article}
\usepackage[utf8]{inputenc}
\usepackage[english]{babel}
\usepackage{csquotes}
\usepackage{amsmath}
\usepackage{amsfonts}
\usepackage{amssymb}
\usepackage{graphicx}
\usepackage[margin=0.5in]{geometry}
\usepackage{amsthm}
\usepackage{enumitem}
\usepackage{tikz}
\usetikzlibrary{calc}
\newtheorem{question}{Question}
\newtheorem*{question*}{Question}
\newtheorem{theorem}{Theorem}
\newtheorem*{theorem*}{Theorem}
\newtheorem{lemma}{Lemma}

\theoremstyle{definition}
\newtheorem{answer}{Answer}
\newtheorem*{answer*}{Answer}


\title{Complex Analysis Homework 5}
\author{Colin Williams}

\begin{document}
\maketitle

\section*{Question 4}
Evaluate 
\begin{align*}
\int_{\gamma} z^m \bar{z}^n dz
\end{align*}
where $m$ and $n$ are integers and $\gamma$ is the unit circle $|z| = 1$ taken counter-clockwise

\begin{answer*}{$ $}
\\I will start by parameterizing $\gamma$ by $\gamma(t) = e^{it}, \; t \in [0, 2\pi]$. Next, note that $\overline{e^{it}} = \overline{\cos(t) + i\sin(t)} = \cos(t) - i\sin(t) = \cos(-t) + i\sin(-t) = e^{-it}$. Thus, using the definition of the path integral:
\begin{align}
\int_{\gamma} z^m\overline{z}^n dz &= \int_0^{2\pi} (e^{it})^m(e^{-it})^n(ie^{it})dt\\
&= i\int_0^{2\pi}e^{(m - n + 1)it}dt\\
&= \frac{i}{i(m - n + 1)}e^{(m - n + 1)it} \big|_{t = 0}^{t = 2\pi}\\
&= \frac{1}{m - n + 1}\left(e^{2\pi i(m - n + 1)} - 1\right)\\
&= 0 \text{ since } m - n + 1 \in \mathbb{Z}
\end{align}
However, this above calculation is only valid whenever $m - n + 1 \neq 0$ i.e. when $m \neq n - 1$. When $m = n - 1$, we have the integral in line (2) reducing to $i\int_0^{2\pi} dt = 2\pi i$. Thus, \boxed{\int_{\gamma} z^m \overline{z}^n dz = 0 \text{ when } m \neq n - 1} and \boxed{\int_{\gamma} z^m \overline{z}^n dz = 2\pi i \text{ when } m = n - 1}
\end{answer*}
\end{document}