\documentclass[10pt,a4paper]{article}
\usepackage[utf8]{inputenc}
\usepackage[english]{babel}
\usepackage{csquotes}
\usepackage{amsmath}
\usepackage{amsfonts}
\usepackage{amssymb}
\usepackage{graphicx}
\usepackage[margin=0.5in]{geometry}
\usepackage{amsthm}
\usepackage{enumitem}
\usepackage{tikz}
\usetikzlibrary{calc}
\newtheorem{question}{Question}
\newtheorem*{question*}{Question}
\newtheorem{theorem}{Theorem}
\newtheorem*{theorem*}{Theorem}
\newtheorem{lemma}{Lemma}

\theoremstyle{definition}
\newtheorem{answer}{Answer}
\newtheorem*{answer*}{Answer}


\title{Complex Analysis Homework 4}
\author{Colin Williams}

\begin{document}
\maketitle

\section*{Question 5}

Evaluate
\[\int_{\gamma} ze^{z^2}dz\]
where $\gamma(t) = i + e^{it}, t \in [-\frac{\pi}{2}, \frac{\pi}{2}]$
\\
\begin{answer*}{$ $}
\\First, let $\displaystyle f(z) = ze^{z^2}$, then note that if $f$ has a primitive (i.e. if there exists some function $F$ such that $F' = f$), then we can evaluate this integral using a familiar analog from real-valued integrals. Namely, 
\[\int_{\gamma} f(z)dz = F(\gamma(b)) - F(\gamma(a))\]
where $a$ and $b$ are defined as the real numbers that specify $\gamma 's$ interval of definition. In other words, $\gamma$ is defined on $[a,b]$. Motivated by the analogous real-valued primitive, I will claim that $F(z) = \frac{1}{2}e^{z^2}$
\\
\\\underline{Proof of claim}
\\I have already shown in Question 1 of this homework assignment that the derivative of $e^{z^2}$ exists and is equal to $2ze^{z^2}$. Therefore, by the property of scalar multiplication on derivatives, we can say that $F'(z) = \frac{1}{2}\cdot \frac{d}{dz}(e^{z^2}) = \frac{1}{2}(2ze^{z^2}) = ze^{z^2}$. Thus, $F$ is, indeed, the primitive of $f$. $\square$
\\
\\With this in place, calculating the above integral is fairly straightforward:
\begin{align*}
\int_{\gamma} ze^{z^2}dz &= F\left(\gamma\left(\frac{\pi}{2}\right)\right) - F\left(\gamma\left(-\frac{\pi}{2}\right)\right)\\
&= F\left(i + e^{i\frac{\pi}{2}}\right) - F\left(i + e^{i(-\frac{\pi}{2})}\right)\\
&= F(2i) - F(0)\\
&= \frac{1}{2}e^{(2i)^2} - \frac{1}{2}e^{0^2}\\
&= \frac{1}{2}(e^{-4} - 1)\\
\implies &\boxed{\int_{\gamma}ze^{z^2} = \frac{1 - e^4}{2e^4} }
\end{align*}
\end{answer*}
\end{document}