\documentclass[10pt,a4paper]{article}
\usepackage[utf8]{inputenc}
\usepackage[english]{babel}
\usepackage{csquotes}
\usepackage{amsmath}
\usepackage{amsfonts}
\usepackage{amssymb}
\usepackage{graphicx}
\usepackage[margin=0.5in]{geometry}
\usepackage{amsthm}
\usepackage{enumitem}
\usepackage{tikz}
\usetikzlibrary{calc}
\newtheorem{question}{Question}
\newtheorem*{question*}{Question}
\newtheorem{theorem}{Theorem}
\newtheorem*{theorem*}{Theorem}
\newtheorem{lemma}{Lemma}

\theoremstyle{definition}
\newtheorem{answer}{Answer}
\newtheorem*{answer*}{Answer}


\title{Complex Analysis Homework 6}
\author{Colin Williams}

\begin{document}
\maketitle

\section*{Question 1}
With the aid of the equalities (for $z = x + iy$),
\begin{align*}
|\sin(z)|^2 = \sin^2(x) + \sinh^2(y), && |\cos(z)|^2 = \cos^2(x) + \sinh^2(y)
\end{align*}
show that
\begin{enumerate}[label = (\alph*)]
\item $|\sinh(y)| \leq |\sin(z)| \leq \cosh(y)$
\item $|\sinh(y)| \leq |\cos(z)| \leq \cosh(y)$
\end{enumerate}

\begin{answer*}{\textbf{(a)}}
\\It is clear from the first equality that $\sinh^2(y) = |\sin(z)|^2 - \sin^2(x)$. Since $\sin(x) \in [-1, 1] \implies \sin^2(x) \in [0,1]$. Thus, $\sin^2(x) \geq 0$ for all $x \in \mathbb{R} \implies -\sin^2(x) \leq 0$ for all $x \in \mathbb{R}$. Thus, using the equality I just found, we get
\begin{align*}
\sinh^2(y) &= |\sin(z)|^2 - \sin^2(x)\\
&\leq |\sin(z)|^2 - 0\\
&= |\sin(z)|^2\\
\implies |\sinh(y)| &\leq |\sin(z)| \quad \text{the first of the two inequalities we need to show}
\end{align*}
Likewise, if we use the fact that $\sinh^2(y) = \cosh^2(y) - 1$, then we get from the first equality that \\$|\sin(z)|^2 = \sin^2(x) + \cosh^2(y) - 1$. Furthermore, using the same analysis on $\sin(x)$ as above, we can determine that $\sin^2(x) \leq 1$ for all $x \in \mathbb{R}$. Thus, putting this together, we get:
\begin{align*}
|\sin(z)|^2 &= \sin^2(x) + \cosh^2(y) - 1\\
&\leq 1 + \cosh^2(y) - 1\\
&= \cosh^2(y)\\
\implies |\sin(z)| &\leq \cosh(y) \quad \text{the second of the two inequalities we need to show}
\end{align*}
Thus, we have now shown that $|\sinh(y)| \leq |\sin(z)| \leq \cosh(y)$, exactly as desired. 
\end{answer*}

\begin{answer*}{\textbf{(b)}}
\\It is clear from the second equality that $\sinh^2(y) = |\cos(z)|^2 - \cos^2(x)$. Since $\cos(x) \in [-1, 1] \implies \cos^2(x) \in [0,1]$. Thus, $\cos^2(x) \geq 0$ for all $x \in \mathbb{R} \implies -\cos^2(x) \leq 0$ for all $x \in \mathbb{R}$. Thus, using the equality I just found, we get
\begin{align*}
\sinh^2(y) &= |\cos(z)|^2 - \cos^2(x)\\
&\leq |\cos(z)|^2 - 0\\
&= |\cos(z)|^2\\
\implies |\sinh(y)| &\leq |\cos(z)| \quad \text{the first of the two inequalities we need to show}
\end{align*}
Likewise, if we use the fact that $\sinh^2(y) = \cosh^2(y) - 1$, then we get from the second equality that \\$|\cos(z)|^2 = \cos^2(x) + \cosh^2(y) - 1$. Furthermore, using the same analysis on $\cos(x)$ as above, we can determine that $\cos^2(x) \leq 1$ for all $x \in \mathbb{R}$. Thus, putting this together, we get:
\begin{align*}
|\cos(z)|^2 &= \cos^2(x) + \cosh^2(y) - 1\\
&\leq 1 + \cosh^2(y) - 1\\
&= \cosh^2(y)\\
\implies |\cos(z)| &\leq \cosh(y) \quad \text{the second of the two inequalities we need to show}
\end{align*}
Thus, we have now shown that $|\sinh(y)| \leq |\cos(z)| \leq \cosh(y)$, exactly as desired. 
\end{answer*}
\end{document}