\documentclass[10pt,a4paper]{article}
\usepackage[utf8]{inputenc}
\usepackage[english]{babel}
\usepackage{amsmath}
\usepackage{amsfonts}
\usepackage{amssymb}
\usepackage{graphicx}
\usepackage[margin=0.5in]{geometry}
\usepackage{amsthm}
\usepackage{enumitem}
\newtheorem{question}{Question}
\newtheorem*{question*}{Question}
\newtheorem{answer}{Answer}
\newtheorem*{answer*}{Answer}
\newtheorem{theorem}{Theorem}
\newtheorem{lemma}{Lemma}

\title{Complex Analysis Homework 3}
\author{Colin Williams}

\begin{document}
\maketitle
\section*{Question 2}
\begin{question*}{$ $}
\\Suppose that $f(z_0) = g(z_0) = 0$ and that $f'(z_0)$ and $g'(z_0)$ exist where $g'(z_0) \neq 0$. Show that
\[\lim_{z \to z_0}\frac{f(z)}{g(z)} = \frac{f'(z_0)}{g'(z_0)}\]
\end{question*}
\begin{proof}{$ $}
\\First, I will examine the left hand side of this equation without the limit:
\begin{align*}
\frac{f(z)}{g(z)} &= \frac{f(z) - f(z_0)}{g(z) - g(z_0)} &\text{since } f(z_0) = g(z_0) = 0\\
&= \frac{f(z) - f(z_0)}{g(z) - g(z_0)} \cdot \frac{\displaystyle \frac{1}{z - z_0}}{\displaystyle \frac{1}{z - z_0}} &\text{since we can multiply by 1}\\
&= \frac{\displaystyle \frac{f(z) - f(z_0)}{z - z_0}}{\displaystyle \frac{g(z) - g(z_0)}{z - z_0}}
\end{align*}
Next, I will make use of the following theorem:
\begin{theorem}{$ $}
\\Suppose that $\displaystyle \lim_{z \to z_0}f(z) = f_0 \text{ and } \lim_{z \to z_0}g(z) = g_0$ with $g_0 \neq 0$, then
\[\lim_{z \to z_0}\frac{f(z)}{g(z)} = \frac{f_0}{g_0}\]
\end{theorem}
I will now take the appropriate limit of $\displaystyle \frac{f(z)}{g(z)}$ as follows:
\begin{align*}
\lim_{z \to z_0} \frac{f(z)}{g(z)} &= \lim_{z \to z_0} \frac{\displaystyle \frac{f(z) - f(z_0)}{z - z_0}}{\displaystyle \frac{g(z) - g(z_0)}{z - z_0}} &\text{by the above calculation.}\\
&= \frac{\displaystyle \lim_{z \to z_0} \frac{f(z) - f(z_0)}{z - z_0}}{\displaystyle \lim_{z \to z_0} \frac{g(z) - g(z_0)}{z - z_0}} &\text{by Theorem 1 and since } \lim_{z \to z_0}\frac{g(z) - g(z_0)}{z - z_0} = g'(z_0) \neq 0 \text{ by assumption}.\\
&= \frac{f'(z_0)}{g'(z_0)} &\text{since we assumed that } f'(z_0) \text{ and } g'(z_0) \text{ exist.}
\end{align*}
Therefore, we have proven the desired statement.
\end{proof}
\end{document}