\documentclass[10pt,a4paper]{article}
\usepackage[utf8]{inputenc}
\usepackage[english]{babel}
\usepackage{csquotes}
\usepackage{amsmath}
\usepackage{amsfonts}
\usepackage{amssymb}
\usepackage{graphicx}
\usepackage[margin=0.5in]{geometry}
\usepackage{amsthm}
\usepackage{enumitem}
\usepackage{tikz}
\usetikzlibrary{calc}
\newtheorem{question}{Question}
\newtheorem*{question*}{Question}
\newtheorem{theorem}{Theorem}
\newtheorem*{theorem*}{Theorem}
\newtheorem{lemma}{Lemma}

\theoremstyle{definition}
\newtheorem{answer}{Answer}
\newtheorem*{answer*}{Answer}


\title{Complex Analysis Homework 4}
\author{Colin Williams}

\begin{document}
\maketitle

\section*{Question 3}

Evaluate $\displaystyle \int_{\gamma} f(z)dz$ when:
\begin{enumerate}[label = (\alph*)]
\item $f(z) = \frac{1}{z}, \gamma(t) = e^{-it}, t \in [0, 8\pi]$
\item $f(z) = $ Re$(z), \gamma(t) = t + it^2, t \in [0,1]$
\item $f(z) = |z|^4, \gamma$ is the line segment $[-1+i, 1 +i]$
\end{enumerate}
$ $
\\First, note the definition of the path integral for a path $\gamma : [a,b] \to \mathbb{C}$ of a function $f: \gamma^* \to \mathbb{C}$:
\begin{equation}
\int_{\gamma}f(z)dz := \int_a^b f(\gamma(t))\gamma '(t)dt
\end{equation}
This makes the calculations pretty straightforward:
\begin{answer*}{\textbf{(a)}}
\\Before we begin, note that $f(\gamma(t)) = e^{it}$ and $\gamma '(t) = -ie^{-it}$; thus, we have
\begin{align*}
\int_{\gamma} f(z)dz &= \int_a^b f(\gamma(t))\gamma '(t)dt &\text{by (1)}\\
&= \int_0^{8\pi} [e^{it}]\cdot[-ie^{-it}]dt &\text{by above comments}\\
&= \int_0^{8\pi} (-i) dt\\
&= -it \Big|_{t = 0}^{t = 8\pi}\\
&= -i(8\pi) - (-i(0))\\
&= \boxed{-8\pi i}
\end{align*}
\end{answer*}

\begin{answer*}{\textbf{(b)}}
\\Before we begin, note that $f(\gamma(t)) = t$ and $\gamma '(t) = 1 + 2it$. Therefore,
\begin{align*}
\int_{\gamma} f(z)dz &= \int_a^b f(\gamma(t))\gamma '(t)dt &\text{by (1)}\\
&= \int_0^1 [t]\cdot[1 + 2it]dt &\text{by the above comments}\\
&= \int_0^1 (t + 2it^2)dt\\
&= \left(\frac{t^2}{2} + \frac{2it^3}{3}\right) \bigg|_{t = 0}^{t = 1}\\
&= \left(\frac{1}{2} + \frac{2i}{3}\right) - (0 + 0)\\
&= \boxed{\frac{1}{2} + \frac{2i}{3}}
\end{align*}
\end{answer*}

\begin{answer*}{\textbf{(c)}}
\\First, let's parameterize $\gamma$ in the following manner: $\gamma(t) = t + i, t \in [-1,1]$. Now, we can see that $\displaystyle f(\gamma(t)) = |\gamma(t)|^4 = \left(\sqrt{t^2 + 1}\right)^4 = (t^2 + 1)^2 = t^4 + 2t^2 + 1$. Furthermore, $\gamma '(t) = 1$, so we can compute the integral as follows:
\begin{align*}
\int_{\gamma} f(z)dz &= \int_a^b f(\gamma(t))\gamma '(t)dt &\text{by (1)}\\
&= \int_{-1}^1 [t^4 + 2t^2 + 1]\cdot[1] dt &\text{by the above comments}\\
&= \int_{-1}^1 (t^4 + 2t^2 + 1) dt\\
&= \left(\frac{t^5}{5} + \frac{2t^3}{3} + t\right) \bigg|_{t = -1}^{t = 1}\\
&= \left(\frac{1}{5} + \frac{2}{3} + 1\right) - \left(\frac{-1}{5} + \frac{-2}{3} - 1\right)\\
&= \frac{2}{5} + \frac{4}{3} + 2\\
&= \boxed{\frac{56}{15}}
\end{align*}
\end{answer*}

\end{document}