\documentclass[10pt,a4paper]{article}
\usepackage[utf8]{inputenc}
\usepackage[english]{babel}
\usepackage{csquotes}
\usepackage{amsmath}
\usepackage{amsfonts}
\usepackage{amssymb}
\usepackage{graphicx}
\usepackage[margin=0.5in]{geometry}
\usepackage{amsthm}
\usepackage{enumitem}
\usepackage{tikz}
\usetikzlibrary{calc}
\newtheorem{question}{Question}
\newtheorem*{question*}{Question}
\newtheorem{theorem}{Theorem}
\newtheorem*{theorem*}{Theorem}
\newtheorem{lemma}{Lemma}

\theoremstyle{definition}
\newtheorem{answer}{Answer}
\newtheorem*{answer*}{Answer}


\title{Complex Analysis Homework 5}
\author{Colin Williams}

\begin{document}
\maketitle

\section*{Question 3}
Evaluate $\displaystyle \int_{\gamma}f(z)dz$ when:
\begin{enumerate}[label = (\alph*)]
\item $f(z)$ is the principal branch 
\begin{align*}
z^i = \exp(i \text{Log}(z)), \quad |z| > 0, \; -\pi < \text{Arg}(z) < \pi
\end{align*}
of the power function $z^i$ and $\gamma(t) = e^{it}$ for $t \in [0,\pi]$.
\item $f(z)$ is the principal branch
\begin{align*}
z^{a-1} = \exp[(a-1) \text{Log}(z)], \quad |z| > 0, \; -\pi < \text{Arg}(z) < \pi
\end{align*}
of the function $z^{a-1}$, where $a \neq 0$ a real number, and $\gamma$ is the positively oriented circle of radius $R > 0$ about the origin.
\end{enumerate}

\begin{answer*}{\textbf{(a)}}
\\I will first use the definition of the path integral:
\begin{align*}
\int_{\gamma} f(z)dz &= \int_0^{\pi} f(\gamma(t))\gamma'(t)dt\\
&= \int_0^{\pi} \left(e^{it}\right)^i (ie^{it})dt\\
&= i\int_0^{\pi} e^{-t}e^{it} dt\\
&= i\int_0^{\pi} e^{(-1 + i)t} dt\\
&= \frac{i}{-1 + i}e^{(-1 + i)t} \Big|_{t = 0}^{t = \pi}\\
&= \frac{i(-1-i)}{(-1 + i)(-1-i)}\left[e^{(-1 + i)\pi} - e^{(-1 + i)0}\right]\\
&= \frac{1 - i}{2} \left[e^{-\pi}e^{i\pi} - 1\right]\\
&= \frac{1 - i}{2}(-e^{-\pi} - 1)\\
&= \frac{-1 + i}{2}(e^{-\pi} + 1)
\end{align*}
Just to be safe, I will calculate it using antiderivatives as well. Note that $\displaystyle \frac{d}{dz}\left(\frac{1}{1 + i}z^{1 + i}\right) = z^i$. However, I will need to change the definition of $f(z)$ to use a different branch of the logarithm function. I will use the branch with $-\frac{\pi}{2} < \text{Arg}(z) < \frac{3\pi}{2}$. Thus, 
\begin{align*}
\int_{\gamma} f(z) dz &= \int_1^{-1} z^i dz\\
&= \left(\frac{1}{1 + i}z^{1 + i}\right) \Big|_{z = 1}^{z = -1}\\
&= \frac{1}{1 + i}\left((-1)^{1 + i} - 1^{1 + i}\right)\\
&= \frac{1}{1 + i}\left( \exp((1 + i)\log(-1)) - \exp((1 + i)\log(1))  \right)\\
&= \frac{1}{1 + i}\left(\exp((1 + i)(\ln(1) + i\pi)) - \exp((1 + i)(\ln(1) - i\cdot 0))\right)\\
&= \frac{1}{1 + i}\left(e^{i\pi}e^{-\pi} - e^0\right)\\
&= \frac{1 - i}{(1 + i)(1 - i)}\left(-e^{-\pi} - 1\right)\\
&= \frac{-1 + i}{2}(e^{-\pi} + 1)
\end{align*}
I got the same answer, so I have verified that \boxed{\int_{\gamma}f(z)dz = \frac{-1 + i}{2}(e^{-\pi} + 1)}
\end{answer*}

\begin{answer*}{\textbf{(b)}}
\\I will first use the definition of the path integral with $\gamma(t) = Re^{it}, \; t \in [-\pi, \pi]$:
\begin{align*}
\int_{\gamma} f(z)dz &= \int_{-\pi}^{\pi} f(\gamma(t))\gamma'(t)dt\\
&= \int_{-\pi}^{\pi} (Re^{it})^{a - 1}(iRe^{it})dt\\
&= iR^a \int_{-\pi}^{\pi} e^{(a - 1)it}e^{it}dt\\
&= iR^a \int_{-\pi}^{\pi} e^{ait}dt\\
&= \frac{iR^a}{ai} e^{ait} \Big|_{t = -\pi}^{t = \pi}\\
&= \frac{R^a}{a}\left(e^{\pi a i} - e^{-\pi ai}\right)\\
&= \frac{R^a}{a}\left(\cos(\pi a) + i\sin(\pi a) - \cos(-\pi a) - i\sin(-\pi a)\right)\\
&= \frac{R^a}{a}2i\sin(\pi a)
\end{align*}
I will check this answer by using antiderivatives as well. Note that $\displaystyle \frac{d}{dz}\left(\frac{1}{a}z^a\right) = z^{a - 1}$ for $a \neq 0$. To do this, I will need to consider two separate branch cuts for two different segments of $\gamma$. Let $\gamma_1 = Re^{it}, \; t \in [-\pi, 0]$, the bottom side of the radius $R$ circle. For this, I will use the branch cut $\log(z) = \ln(|z|) + i\text{Arg}(z), \; -\frac{3\pi}{2} < \text{Arg}(z) < \frac{\pi}{2}$:
\begin{align*}
\int_{\gamma_1} f(z) dz &= \int_{-R}^{R} z^{a - 1}dz\\
&= \frac{1}{a}z^a \Big|_{z = -R}^{z = R}\\
&= \frac{1}{a}\left((R)^a - (-R)^a\right)\\
&= \frac{1}{a}\left(e^{a\text{Log}(R)} - e^{a\text{Log}(-R)}\right)\\
&= \frac{1}{a}\left(e^{a(\ln(R) + i \cdot 0)} - e^{a(\ln(R) - \pi i}\right)\\
&= \frac{1}{a}e^{a\ln(R)}\left(1 - e^{-\pi ai}\right)\\
&= \frac{R^a}{a}e^{-\pi ai}\left(e^{\pi ai} - 1\right)
\end{align*}
Next, I will define $\gamma_2 = Re^{it}, \; t \in [0, \pi]$. For this, I will use the branch cut for $\log(z) = \ln(|z|) + i\text{Arg}(z), \; -\frac{\pi}{2} < \text{Arg}(z) < \frac{3\pi}{2}$ and find that:
\begin{align*}
\int_{\gamma_2}f(z) dz &= \int_{R}^{-R} z^{a - 1} dz\\
&= \frac{1}{a}z^a \Big|_{z = R}^{z = -R}\\
&= \frac{1}{a}\left((-R)^a - (R)^a\right)\\
&= \frac{1}{a}\left(e^{a\text{Log}(-R)} - e^{a\text{Log}(R)}\right)\\
&= \frac{1}{a}\left(e^{a(\ln(R) + \pi i)} - e^{a(\ln(R) + i \cdot 0)}\right)\\
&= \frac{1}{a}e^{a\ln(R)}\left(e^{\pi ai} - 1\right)\\
&= \frac{R^a}{a}\left(e^{\pi ai} - 1\right)
\end{align*}
Therefore, we can calculate the total integral as:
\begin{align*}
\int_{\gamma} f(z)dz &= \int_{\gamma_1}f(z)dz + \int_{\gamma_2}f(z)dz\\
&= \left[\frac{R^a}{a}e^{-\pi ai}\left(e^{\pi ai} - 1\right)\right] + \left[\frac{R^a}{a}\left(e^{\pi ai} - 1\right)\right]\\
&= \frac{R^a}{a}\left(e^{\pi ai} - 1\right)\left(e^{-\pi ai} + 1\right)\\
&= \frac{R^a}{a}\left(e^{\pi a i} - e^{-\pi ai}\right)\\
&= \frac{R^a}{a}2i\sin(\pi a)
\end{align*}
Thus, the two answers are the same, so \boxed{\int_{\gamma} f(z)dz = \frac{R^a}{a}2i\sin(\pi a)}
\end{answer*}

\end{document}